wip

Matroid/Connectivity/Separation.lean
@@ -1,6 +1,7 @@
 import Matroid.Connectivity.Core
 import Matroid.Connectivity.Nat
 import Matroid.Connectivity.Connected
+import Matroid.Connectivity.Minor
 import Matroid.ForMathlib.Finset
 import Matroid.ForMathlib.Matroid.Sum
 
@@ -335,6 +336,144 @@ lemma union_symm (P Q : M.Partition) : (P.union Q).symm = P.symm.inter Q.symm :=
 
 end Cross
 
+section Minor
+
+variable {C D : Set α} {e f : α}
+
+@[simp]
+lemma disjoint_left_contract (P : (M ／ C).Partition) : Disjoint P.left C := by
+  grw [P.left_subset_ground]
+  exact disjoint_sdiff_left
+
+@[simp]
+lemma disjoint_right_contract (P : (M ／ C).Partition) : Disjoint P.right C :=
+  P.symm.disjoint_left_contract
+
+@[simp]
+lemma disjoint_left_delete (P : (M ＼ D).Partition) : Disjoint P.left D := by
+  grw [P.left_subset_ground]
+  exact disjoint_sdiff_left
+
+@[simp]
+lemma disjoint_right_delete (P : (M ＼ D).Partition) : Disjoint P.right D :=
+  P.symm.disjoint_left_delete
+
+@[simps!]
+def contractDual (P : (M ／ C).Partition) : (M✶ ＼ C).Partition := P.dual.copy rfl
+
+@[simps!]
+def deleteDual (P : (M ＼ D).Partition) : (M✶ ／ D).Partition := P.dual.copy rfl
+
+/-- Extend a partition of `M ／ C` to a partition of `M` by adding `C` to the left side. -/
+@[simps]
+def ofContractLeft (P : (M ／ C).Partition) (hC : C ⊆ M.E := by aesop_mat) : M.Partition where
+  left := P.left ∪ C
+  right := P.right
+  disjoint := by simp [P.disjoint_right_contract.symm, P.disjoint]
+  union_eq := by rw [union_right_comm, P.union_eq, contract_ground, diff_union_of_subset hC]
+
+/-- Extend a partition of `M ／ C` to a partition of `M` by adding `C` to the right side. -/
+@[simps!]
+def ofContractRight (P : (M ／ C).Partition) (hC : C ⊆ M.E := by aesop_mat) :=
+  P.symm.ofContractLeft.symm
+
+/-- Extend a partition of `M ＼ D` to a partition of `M` by adding `D` to the left side. -/
+@[simps]
+def ofDeleteLeft (P : (M ＼ D).Partition) (hC : D ⊆ M.E := by aesop_mat) : M.Partition where
+  left := P.left ∪ D
+  right := P.right
+  disjoint := by simp [P.disjoint_right_delete.symm, P.disjoint]
+  union_eq := by rw [union_right_comm, P.union_eq, delete_ground, diff_union_of_subset hC]
+
+/-- Extend a partition of `M ＼ D` to a partition of `M` by adding `D` to the right side. -/
+@[simps!]
+def ofDeleteRight (P : (M ＼ D).Partition) (hD : D ⊆ M.E := by aesop_mat) :=
+  P.symm.ofDeleteLeft.symm
+
+@[simp]
+lemma ofDeleteLeft_symm (P : (M ＼ D).Partition) (hD : D ⊆ M.E := by aesop_mat) :
+    P.ofDeleteLeft.symm = P.symm.ofDeleteRight := rfl
+
+@[simp]
+lemma ofDeleteRight_symm (P : (M ＼ D).Partition) (hD : D ⊆ M.E := by aesop_mat) :
+    P.ofDeleteRight.symm = P.symm.ofDeleteLeft := rfl
+
+@[simp]
+lemma ofContractLeft_symm (P : (M ／ C).Partition) (hC : C ⊆ M.E := by aesop_mat) :
+    P.ofContractLeft.symm = P.symm.ofContractRight := rfl
+
+@[simp]
+lemma ofContractRight_symm (P : (M ／ C).Partition) (hC : C ⊆ M.E := by aesop_mat) :
+    P.ofContractRight.symm = P.symm.ofContractLeft := rfl
+
+@[simp]
+lemma ofDeleteLeft_dual (P : (M ＼ D).Partition) (hD : D ⊆ M.E := by aesop_mat) :
+    P.ofDeleteLeft.dual = P.deleteDual.ofContractLeft := rfl
+
+@[simp]
+lemma ofDeleteRight_dual (P : (M ＼ D).Partition) (hD : D ⊆ M.E := by aesop_mat) :
+    P.ofDeleteRight.dual = P.deleteDual.ofContractRight := rfl
+
+@[simp]
+lemma ofContractLeft_dual (P : (M ／ C).Partition) (hC : C ⊆ M.E := by aesop_mat) :
+    P.ofContractLeft.dual = P.contractDual.ofDeleteLeft := rfl
+
+@[simp]
+lemma ofContractRight_dual (P : (M ／ C).Partition) (hC : C ⊆ M.E := by aesop_mat) :
+    P.ofContractRight.dual = P.contractDual.ofDeleteRight := rfl
+
+lemma compl_left_delete (P : (M ＼ D).Partition) (hD : D ⊆ M.E := by aesop_mat) :
+    M.E \ P.left = P.right ∪ D := by
+  grw [← P.compl_left, delete_ground, diff_diff_comm, diff_union_self, eq_comm, union_eq_left,
+    subset_diff, and_iff_right hD, P.left_subset_ground]
+  exact disjoint_sdiff_right
+
+lemma compl_right_delete (P : (M ＼ D).Partition) (hD : D ⊆ M.E := by aesop_mat) :
+    M.E \ P.right = P.left ∪ D :=
+  P.symm.compl_left_delete
+
+lemma compl_left_contract (P : (M ／ C).Partition) (hD : C ⊆ M.E := by aesop_mat) :
+    M.E \ P.left = P.right ∪ C :=  by
+  simpa using (P.dual.copy (show (M ／ C)✶.E = (M✶ ＼ C).E by simp)).compl_left_delete
+
+lemma compl_right_contract (P : (M ／ C).Partition) (hD : C ⊆ M.E := by aesop_mat) :
+    M.E \ P.right = P.left ∪ C :=
+  P.symm.compl_left_contract
+
+lemma compl_left_delete_singleton (P : (M ＼ {e}).Partition) (he : e ∈ M.E := by aesop_mat) :
+    M.E \ P.left = insert e P.right := by
+  simp [P.compl_left_delete]
+
+lemma compl_right_delete_singleton (P : (M ＼ {e}).Partition) (he : e ∈ M.E := by aesop_mat) :
+    M.E \ P.right = insert e P.left :=
+  P.symm.compl_left_delete_singleton
+
+lemma compl_left_contract_singleton (P : (M ／ {e}).Partition) (he : e ∈ M.E := by aesop_mat) :
+    M.E \ P.left = insert e P.right := by
+  simp [P.compl_left_contract]
+
+@[simp]
+lemma compl_right_contract_singleton (P : (M ／ {e}).Partition) (he : e ∈ M.E := by aesop_mat) :
+    M.E \ P.right = insert e P.left :=
+  P.symm.compl_left_contract_singleton
+
+lemma ofContractLeft_eConn (P : (M ／ C).Partition) (hC : C ⊆ M.E := by aesop_mat) :
+    P.ofContractLeft.eConn = P.eConn + M.eLocalConn P.right C := by
+  simp only [← eConn_left, ofContractLeft_left]
+  rw [eConn_union_eq_eConn_contract_add _ P.disjoint_left_contract, ← P.compl_right_contract,
+    diff_diff_cancel_left]
+  grw [P.right_subset_ground, contract_ground, diff_subset]
+
+lemma ofContractRight_eConn (P : (M ／ C).Partition) (hC : C ⊆ M.E := by aesop_mat) :
+    P.ofContractRight.eConn = P.eConn + M.eLocalConn P.left C := by
+  rw [← eConn_symm, P.ofContractRight_symm, ofContractLeft_eConn, eConn_symm, symm_right]
+
+
+
+
+
+end Minor
+
 
 lemma eConn_eq_zero_iff_skew {P : M.Partition} : P.eConn = 0 ↔ M.Skew P.1 P.2 :=
   M.eLocalConn_eq_zero P.left_subset_ground P.right_subset_ground
@@ -394,256 +533,3 @@ protected lemma wlog_symm_dual (motive : {N : Matroid α} → (P : N.Partition) 
 end wlog
 
 end Partition
-
-@[mk_iff]
-structure Partition.SepOf (P : M.Partition) (X Y : Set α) : Prop where
-  subset_left : X ⊆ P.left
-  subset_right : Y ⊆ P.right
-
-lemma Partition.sepOf_iff_left (P : M.Partition) (hY : Y ⊆ M.E) :
-    P.SepOf X Y ↔ X ⊆ P.left ∧ Disjoint P.left Y := by
-  rw [sepOf_iff, ← P.compl_left, subset_diff, and_iff_right hY, disjoint_comm]
-
-lemma Partition.sepOf_iff_right (P : M.Partition) (hX : X ⊆ M.E) :
-    P.SepOf X Y ↔ Disjoint X P.right ∧ Y ⊆ P.right := by
-  rw [sepOf_iff, ← P.compl_right, subset_diff, and_iff_right hX]
-
-lemma Partition.SepOf.symm (hP : P.SepOf X Y) : P.symm.SepOf Y X :=
-  ⟨hP.2, hP.1⟩
-
-lemma Partition.SepOf.disjoint (hP : P.SepOf X Y) : Disjoint X Y :=
-  P.disjoint.mono hP.1 hP.2
-
-lemma Partition.SepOf.mono_left (hP : P.SepOf X Y) (hX'X : X' ⊆ X) : P.SepOf X' Y :=
-  ⟨hX'X.trans hP.1, hP.2⟩
-
-lemma Partition.SepOf.mono_right (hP : P.SepOf X Y) (hY'Y : Y' ⊆ Y) : P.SepOf X Y' :=
-  ⟨hP.1, hY'Y.trans hP.2⟩
-
-lemma Partition.SepOf.disjoint_left (hP : P.SepOf X Y) : Disjoint P.left Y :=
-  (subset_diff.1 <| hP.subset_right.trans_eq P.compl_left.symm).2.symm
-
-lemma Partition.SepOf.disjoint_right (hP : P.SepOf X Y) : Disjoint X P.right :=
-  (subset_diff.1 <| hP.subset_left.trans_eq P.compl_right.symm).2
-
-lemma Partition.SepOf.mono (hP : P.SepOf X Y) (hX'X : X' ⊆ X) (hY'Y : Y' ⊆ Y) : P.SepOf X' Y' :=
-  ⟨hX'X.trans hP.1, hY'Y.trans hP.2⟩
-
-@[simp]
-lemma Partition.symm_sepOf_iff : P.symm.SepOf X Y ↔ P.SepOf Y X :=
-  ⟨fun h ↦ h.symm, fun h ↦ h.symm⟩
-
-lemma partition_sepOf (hXY : Disjoint X Y) (hXE : X ⊆ M.E) (hYE : Y ⊆ M.E) :
-    (M.partition X).SepOf X Y := by
-  rw [Partition.sepOf_iff_left _ hYE, partition_left _ _ hXE, and_iff_left hXY]
-
-
--- lemma Partition.restrict_sepOf_iff (R : Set α) :
---     (P.restrict R).SepOf X Y ↔ P.SepOf X Y ∧ X ⊆ R ∧ Y ⊆ R := by
---   simp only [SepOf, restrict_left, subset_inter_iff, restrict_right]
---   refine ⟨fun ⟨⟨h1, h2⟩, h3⟩ ↦ ?_, fun h ↦ ?_⟩
---   · refine ⟨⟨h1, ?_⟩, ?_⟩
-
-lemma Partition.SepOf.left_subset_ground (h : P.SepOf X Y) : X ⊆ M.E :=
-  h.1.trans P.left_subset_ground
-
-lemma Partition.SepOf.right_subset_ground (h : P.SepOf X Y) : Y ⊆ M.E :=
-  h.2.trans P.right_subset_ground
-
-lemma Partition.sepOf_self_compl_iff (hX : X ⊆ M.E) :
-    P.SepOf X (M.E \ X) ↔ P = M.partition X hX := by
-  rw [sepOf_iff, diff_subset_comm, P.compl_right, ← subset_antisymm_iff]
-  refine ⟨?_, by simp +contextual⟩
-  rintro rfl
-  exact Partition.ext rfl <| by simp [P.compl_left]
-
-lemma Partition.sepOf_compl_self_iff (hX : X ⊆ M.E) :
-    P.SepOf (M.E \ X) X ↔ P = M.partition (M.E \ X) diff_subset := by
-  rw [← sepOf_self_compl_iff]
-  simp [inter_eq_self_of_subset_right hX]
-
-/-- The minimum order of a separation of `M` with `X` and `Y` contained in different sides.
-The 'well-defined' inputs are where `X` and `Y` are disjoint subsets of `M.E`,
-but we give a more complicated definition (in terms of `Matroid.core`)
-that ignores junk elements, loops and coloops in `X` and `Y`.
-This definition is the simplest definition that is unconditionally monotone under restrictions,
-and preserved by intersections with the ground set, duality and adding/removing loops.
-`Matroid.eConnBetween_eq_iInf` shows that the definition behaves correctly for sensible inputs. -/
-noncomputable def eConnBetween (M : Matroid α) (X Y : Set α) : ℕ∞ :=
-  ⨅ P : {P : M.Partition // P.SepOf (M.core X) (M.core Y)}, P.1.eConn
-
-lemma Partition.SepOf.eConnBetween_le_of_core (hP : P.SepOf (M.core X) (M.core Y)) :
-    M.eConnBetween X Y ≤ P.eConn :=
-  iInf_le_of_le ⟨P, hP⟩ rfl.le
-
-lemma Partition.SepOf.eConnBetween_le (hP : P.SepOf X Y) :
-    M.eConnBetween X Y ≤ P.eConn :=
-  (hP.mono (M.core_subset X) (M.core_subset Y)).eConnBetween_le_of_core
-
-lemma eConnBetween_symm (M : Matroid α) : M.eConnBetween X Y = M.eConnBetween Y X := by
-  apply le_antisymm <;>
-  exact le_iInf fun ⟨P, hP⟩ ↦ iInf_le_of_le ⟨P.symm, by simpa⟩ (by simp)
-
-lemma eConnBetween_le_eConn_left (M : Matroid α) (hdj : Disjoint X Y) :
-    M.eConnBetween X Y ≤ M.eConn X := by
-  have h : (M.partition (M.core X)).SepOf (M.core X) (M.core Y) := by
-    simpa [Partition.sepOf_iff, subset_diff] using hdj.symm.mono (core_subset ..) (core_subset ..)
-  exact h.eConnBetween_le_of_core.trans <| by simp
-
-lemma eConnBetween_le_eConn_right (M : Matroid α) (hdj : Disjoint X Y) :
-    M.eConnBetween X Y ≤ M.eConn Y := by
-  rw [eConnBetween_symm]
-  exact M.eConnBetween_le_eConn_left hdj.symm
-
-lemma le_eConnBetween_iff_forall_sepOf_core {k : ℕ∞} : k ≤ M.eConnBetween X Y ↔
-    ∀ (P : M.Partition), P.SepOf (M.core X) (M.core Y) → k ≤ P.eConn := by
-  simp [eConnBetween, le_iInf_iff, Subtype.forall]
-
-lemma eConnBetween_eq_iInf (hXY : Disjoint X Y) (hX : X ⊆ M.E) (hY : Y ⊆ M.E) :
-    M.eConnBetween X Y = ⨅ P : {P : M.Partition // P.SepOf X Y}, P.1.eConn := by
-  simp only [eConnBetween, le_antisymm_iff, le_iInf_iff, Subtype.forall]
-  refine ⟨fun P hP ↦ ?_, fun P hP ↦ ?_⟩
-  · exact iInf_le_of_le ⟨P, hP.mono (M.core_subset X) (M.core_subset Y)⟩ rfl.le
-  refine iInf_le_of_le ⟨M.partition ((P.left ∪ X) \ Y), ?_⟩ ?_
-  · simpa [Partition.sepOf_iff_left _ hY, disjoint_sdiff_left, subset_diff]
-  rw [eConn_partition, ← eConn_core, core_diff, core_union, ← M.core_core X,
-    union_eq_self_of_subset_right (M.core_subset_core hP.1), sdiff_eq_left.2, eConn_core,
-    P.eConn_left]
-  exact hP.disjoint_left.mono_left (M.core_subset ..)
-
-lemma le_eConnBetween_iff_forall_sepOf {k : ℕ∞} (hdj : Disjoint X Y) (hX : X ⊆ M.E) (hY : Y ⊆ M.E) :
-    k ≤ M.eConnBetween X Y ↔ ∀ (P : M.Partition), P.SepOf X Y → k ≤ P.eConn := by
-  simp [eConnBetween_eq_iInf hdj hX hY]
-
-lemma exists_partition_eConn_eq_eConnBetween_core (hXY : Disjoint (M.core X) (M.core Y)) :
-    ∃ P : M.Partition, P.SepOf (M.core X) (M.core Y) ∧ P.eConn = M.eConnBetween X Y := by
-  set α := {P : M.Partition // P.SepOf (M.core X) (M.core Y)}
-  have hne : Nonempty α := ⟨_, partition_sepOf hXY (core_subset_ground ..) (core_subset_ground ..)⟩
-  obtain ⟨⟨P,h⟩, hP⟩ := ENat.exists_eq_iInf (f := fun i : α ↦ i.1.eConn)
-  exact ⟨P, h, hP⟩
-
-lemma exists_partition_eConn_eq_eConnBetween (hXY : Disjoint X Y) (hXE : X ⊆ M.E) (hYE : Y ⊆ M.E) :
-    ∃ P : M.Partition, P.SepOf X Y ∧ P.eConn = M.eConnBetween X Y := by
-  simp_rw [eConnBetween_eq_iInf hXY hXE hYE]
-  set α := {P : M.Partition // P.SepOf X Y}
-  have hne : Nonempty α := ⟨_, partition_sepOf hXY hXE hYE⟩
-  obtain ⟨⟨P,h⟩, hP⟩ := ENat.exists_eq_iInf (f := fun i : α ↦ i.1.eConn)
-  exact ⟨P, h, hP⟩
-
-lemma eConnBetween_of_not_disjoint (M : Matroid α) (hXY : ¬ Disjoint (M.core X) (M.core Y)) :
-    M.eConnBetween X Y = ⊤ := by
-  simp [eConnBetween, iInf_subtype, show ∀ P : M.Partition, ¬ P.SepOf (M.core X) (M.core Y) from
-    fun P hP ↦ hXY <| P.disjoint.mono hP.1 hP.2]
-
-lemma eConnBetween_mono_left (M : Matroid α) (hX : X' ⊆ X) (Y : Set α) :
-    M.eConnBetween X' Y ≤ M.eConnBetween X Y :=
-  le_iInf fun ⟨P, hP⟩ ↦ iInf_le_of_le ⟨P, hP.mono_left (M.core_subset_core hX)⟩ rfl.le
-
-lemma eConnBetween_mono_right (M : Matroid α) (X : Set α) (hY : Y' ⊆ Y) :
-    M.eConnBetween X Y' ≤ M.eConnBetween X Y :=
-  le_iInf fun ⟨P, hP⟩ ↦ iInf_le_of_le ⟨P, hP.mono_right (M.core_subset_core hY)⟩ rfl.le
-
-lemma eConnBetween_mono (M : Matroid α) (hX : X' ⊆ X) (hY : Y' ⊆ Y) :
-    M.eConnBetween X' Y' ≤ M.eConnBetween X Y :=
-  (M.eConnBetween_mono_left hX _).trans <| M.eConnBetween_mono_right _ hY
-
-@[simp]
-lemma eConnBetween_core_left (M : Matroid α) (X Y : Set α) :
-    M.eConnBetween (M.core X) Y = M.eConnBetween X Y := by
-  simp [eConnBetween, iInf_subtype]
-
-@[simp]
-lemma eConnBetween_core_right (M : Matroid α) (X Y : Set α) :
-    M.eConnBetween X (M.core Y) = M.eConnBetween X Y := by
-  simp [eConnBetween, iInf_subtype]
-
-@[simp]
-lemma eConnBetween_inter_ground_left (M : Matroid α) (X Y : Set α) :
-    M.eConnBetween (X ∩ M.E) Y = M.eConnBetween X Y := by
-  refine (M.eConnBetween_mono_left inter_subset_left _).antisymm ?_
-  rw [← eConnBetween_core_left]
-  exact M.eConnBetween_mono_left (by simp) _
-
-@[simp]
-lemma eConnBetween_inter_ground_right (M : Matroid α) (X Y : Set α) :
-    M.eConnBetween X (Y ∩ M.E) = M.eConnBetween X Y := by
-  rw [eConnBetween_symm, eConnBetween_inter_ground_left, eConnBetween_symm]
-
-@[simp]
-lemma eConnBetween_self_compl (M : Matroid α) (X : Set α) :
-    M.eConnBetween X (M.E \ X) = M.eConn X := by
-  wlog hXE : X ⊆ M.E generalizing X with aux
-  · rw [← eConnBetween_inter_ground_left, ← diff_inter_self_eq_diff, aux _ inter_subset_right,
-      eConn_inter_ground]
-  obtain ⟨P, hP, hP'⟩ := exists_partition_eConn_eq_eConnBetween disjoint_sdiff_right hXE diff_subset
-  rw [Partition.sepOf_self_compl_iff hXE] at hP
-  rw [← hP', hP, eConn_partition]
-
-@[simp]
-lemma eConnBetween_compl_self (M : Matroid α) (X : Set α) :
-    M.eConnBetween (M.E \ X) X = M.eConn X := by
-  rw [eConnBetween_symm, M.eConnBetween_self_compl]
-
-@[simp]
-lemma eConnBetween_dual_eq (M : Matroid α) (X Y : Set α) :
-    M✶.eConnBetween X Y = M.eConnBetween X Y := by
-  simp only [eConnBetween, iInf_subtype, core_dual]
-  apply (Partition.dualEquiv M).symm.iInf_congr
-  intro P
-  convert rfl using 2 <;>
-  simp [Partition.sepOf_iff]
-
-@[simp]
-lemma eConnBetween_removeLoops_eq (M : Matroid α) :
-    M.removeLoops.eConnBetween = M.eConnBetween := by
-  ext X Y
-  obtain hndj | hdj := em' <| Disjoint (M.core X) (M.core Y)
-  · rw [eConnBetween_of_not_disjoint _ (by simpa), eConnBetween_of_not_disjoint _ hndj]
-  refine le_antisymm ?_ ?_
-  · obtain ⟨P, hP, hP_eq⟩ := M.exists_partition_eConn_eq_eConnBetween_core hdj
-    refine iInf_le_of_le ⟨M.removeLoops.partition (P.left ∩ _) inter_subset_right, ?_⟩ ?_
-    · rw [Partition.sepOf_iff_left _ (core_subset_ground ..)]
-      simp only [removeLoops_core, partition_left, subset_inter_iff, hP.1, true_and]
-      rw [← removeLoops_core, and_iff_right (core_subset_ground ..)]
-      exact P.disjoint.mono inter_subset_left hP.2
-    simp only [eConn_partition, removeLoops_eConn, ← hP_eq, ← P.eConn_left]
-    rw [← removeLoops_eConn, eConn_inter_ground]
-  obtain ⟨P, hP, hP_eq⟩ := M.removeLoops.exists_partition_eConn_eq_eConnBetween_core (by simpa)
-  refine iInf_le_of_le ⟨M.partition P.left ?_, ?_⟩ ?_
-  · exact P.left_subset_ground.trans M.removeLoops_isRestriction.subset
-  · rw [Partition.sepOf_iff_left _ (by simp)]
-    simp only [partition_left]
-    simp only [removeLoops_core] at hP
-    exact ⟨hP.1, hP.disjoint_left⟩
-  simp only [eConn_partition, hP_eq.symm, ← P.eConn_left, removeLoops_eConn]
-  exact rfl.le
-
-lemma eConnBetween_restrict_le (M : Matroid α) (X Y R : Set α) :
-    (M ↾ R).eConnBetween X Y ≤ M.eConnBetween X Y := by
-  wlog hRE : R ⊆ M.E with aux
-  · rw [← eConnBetween_removeLoops_eq, restrict_removeLoops, eConnBetween_removeLoops_eq]
-    exact aux M X Y (R ∩ M.E) inter_subset_right
-  rw [le_eConnBetween_iff_forall_sepOf_core]
-  intro P hP
-  refine iInf_le_of_le ⟨P.restrict R, ?_⟩ ?_
-  · rw [Partition.sepOf_iff_left _ (core_subset_ground ..)]
-    simp only [Partition.restrict_left, subset_inter_iff]
-    exact ⟨⟨(core_restrict_subset ..).trans hP.1, core_subset_ground ..⟩,
-      P.disjoint.mono inter_subset_left ((core_restrict_subset ..).trans hP.2)⟩
-  simp only [eLocalConn_restrict_eq, Partition.restrict_left, inter_assoc, inter_self,
-    Partition.restrict_right, diff_eq_empty.2 hRE, union_empty, Partition.eConn]
-  exact M.eLocalConn_mono inter_subset_left inter_subset_left
-
-lemma eConnBetween_delete_le (M : Matroid α) (X Y D : Set α) :
-    (M ＼ D).eConnBetween X Y ≤ M.eConnBetween X Y := by
-  apply eConnBetween_restrict_le
-
-lemma eConnBetween_contract_le (M : Matroid α) (X Y C : Set α) :
-    (M ／ C).eConnBetween X Y ≤ M.eConnBetween X Y := by
-  rw [← eConnBetween_dual_eq, dual_contract, ← M.eConnBetween_dual_eq]
-  apply eConnBetween_delete_le
-
-lemma IsMinor.eConnBetween_le {N : Matroid α} (hNM : N ≤m M) :
-    N.eConnBetween X Y ≤ M.eConnBetween X Y := by
-  obtain ⟨C, D, h, -, -, rfl⟩ := hNM
-  exact le_trans ((M ／ C).eConnBetween_delete_le X Y D) <| (M.eConnBetween_contract_le X Y C)
